plf/Equiv.v
@@ -123,7 +123,7 @@ Theorem bequiv_example:
     <{ X - X = 0 }>
     <{ true }>.
 Proof.
-  unfold bequiv. intros st. unfold beval.
+  intros st. unfold beval.
   rewrite aequiv_example. reflexivity.
 Qed.
 
@@ -142,8 +142,6 @@ Qed.
 Definition cequiv (c1 c2 : com) : Prop :=
   forall (st st' : state),
     (st =[ c1 ]=> st') <-> (st =[ c2 ]=> st').
-
-Locate ceval.
 
 (** We can also define an asymmetric variant of this relation: We say
     that [c1] _refines_ [c2] if they produce the same final states
@@ -187,9 +185,15 @@ Theorem skip_right : forall c,
   cequiv
     <{ c ; skip }>
     c.
-Proof. Admitted.
-
-(** Similarly, here is a simple equivalence that optimizes [if]
+Proof.
+  unfold cequiv. split.
+  - intro H. inversion H; subst.
+    inversion H5; subst.
+     assumption.
+  - intro H. apply E_Seq with (st'). * assumption.
+    * apply E_Skip.
+Qed.
+    (** Similarly, here is a simple equivalence that optimizes [if]
     commands: *)
 
 Theorem if_true_simple : forall c1 c2,
@@ -278,8 +282,17 @@ Theorem if_false : forall b c1 c2,
     <{ if b then c1 else c2 end }>
     c2.
 Proof.
-  (* FILL IN HERE *) Admitted.
-(** [] *)
+ intros b c1 c2 Hb.
+  split; intros H.
+  - (* -> *)
+    inversion H; subst.
+    + unfold bequiv in Hb. simpl in Hb.
+      rewrite Hb in H5. discriminate.
+    + assumption.
+  - apply E_IfFalse. 
+    + unfold bequiv in Hb. auto.
+    + assumption.
+Qed.
 
 (** **** Exercise: 3 stars, standard (swap_if_branches)
 
@@ -291,8 +304,18 @@ Theorem swap_if_branches : forall b c1 c2,
     <{ if b then c1 else c2 end }>
     <{ if ~ b then c2 else c1 end }>.
 Proof.
-  (* FILL IN HERE *) Admitted.
-(** [] *)
+  unfold cequiv; split; intro H.
+  - inversion H; subst. 
+    + apply E_IfFalse.
+      * simpl; apply negb_false_iff; assumption.
+      * assumption.
+    + apply E_IfTrue. 
+      * simpl. apply negb_true_iff; assumption.
+      * assumption.
+  - inversion H; subst.
+    + simpl in H5; apply negb_true_iff in H5; apply E_IfFalse; assumption.
+    + simpl in H5; apply negb_false_iff in H5; apply E_IfTrue; assumption.
+Qed. 
 
 (** For [while] loops, we can give a similar pair of theorems.  A loop
     whose guard is equivalent to [false] is equivalent to [skip],
@@ -394,8 +417,10 @@ Theorem while_true : forall b c,
     <{ while b do c end }>
     <{ while true do skip end }>.
 Proof.
-  (* FILL IN HERE *) Admitted.
-(** [] *)
+intros b c Hb st st'.
+  split; intros H; apply while_true_nonterm in H; exfalso; try assumption;
+  apply while_true_nonterm in H; try assumption. unfold bequiv; reflexivity.
+Qed.
 
 (** A more interesting fact about [while] commands is that any number
     of copies of the body can be "unrolled" without changing meaning.
@@ -438,8 +463,15 @@ Proof.
 Theorem seq_assoc : forall c1 c2 c3,
   cequiv <{(c1;c2);c3}> <{c1;(c2;c3)}>.
 Proof.
-  (* FILL IN HERE *) Admitted.
-(** [] *)
+  split; intro H; inversion H; subst.
+  - inversion H2; subst.
+    apply E_Seq with (st':=st'1); try assumption.
+    apply E_Seq with (st':=st'0); try assumption.
+  - inversion H5; subst.
+    apply E_Seq with st'1.
+    + apply E_Seq with st'0; assumption.
+    + assumption.
+Qed.
 
 (** Proving program properties involving assignments is one place
     where the fact that program states are treated extensionally
@@ -467,8 +499,14 @@ Theorem assign_aequiv : forall (X : string) (a : aexp),
   aequiv <{ X }> a ->
   cequiv <{ skip }> <{ X := a }>.
 Proof.
-  (* FILL IN HERE *) Admitted.
-(** [] *)
+intros X a Ha.
+  unfold aequiv in Ha.
+  split; intro H; inversion H; subst; clear H.
+  - assert (H : st' =[ X := a ]=> (X !-> st' X ; st')).
+  { constructor. rewrite <- Ha. reflexivity. }
+    rewrite t_update_same in H. assumption.
+  - rewrite <- (Ha st). rewrite t_update_same. constructor.
+Qed.
 
 (** **** Exercise: 2 stars, standard (equiv_classes) *)
 
@@ -725,8 +763,14 @@ Theorem CSeq_congruence : forall c1 c1' c2 c2',
   cequiv c1 c1' -> cequiv c2 c2' ->
   cequiv <{ c1;c2 }> <{ c1';c2' }>.
 Proof.
-  (* FILL IN HERE *) Admitted.
-(** [] *)
+  split; intros H1; inversion H1; subst.
+  - apply E_Seq with st'0. 
+    + apply H; assumption.
+    + apply H0; assumption.
+  - apply E_Seq with st'0. 
+    + apply H; assumption.
+    + apply H0; assumption.
+Qed.
 
 (** **** Exercise: 3 stars, standard (CIf_congruence) *)
 Theorem CIf_congruence : forall b b' c1 c1' c2 c2',
@@ -734,10 +778,22 @@ Theorem CIf_congruence : forall b b' c1 c1' c2 c2',
   cequiv <{ if b then c1 else c2 end }>
          <{ if b' then c1' else c2' end }>.
 Proof.
-  (* FILL IN HERE *) Admitted.
-(** [] *)
+  split; intro H2. 
+  - inversion H2; subst. 
+    +  apply E_IfTrue. 
+      { rewrite <- H; assumption. }
+      apply H0; assumption.
+    + apply E_IfFalse. { rewrite <- H; assumption. }
+      apply H1; assumption.
+  - inversion H2; subst. 
+    +  apply E_IfTrue. 
+      { rewrite H; assumption. }
+      apply H0; assumption.
+    + apply E_IfFalse. { rewrite H; assumption. }
+      apply H1; assumption.
+Qed.
 
-(** For example, here are two equivalent programs and a proof of their
+      (** For example, here are two equivalent programs and a proof of their
     equivalence using these congruence theorems... *)
 
 Example congruence_example:
@@ -1115,9 +1171,25 @@ Proof.
        become constants after folding *)
       simpl. destruct (n =? n0); reflexivity.
   - (* BLe *)
-    (* FILL IN HERE *) admit.
+    simpl.
+    remember (fold_constants_aexp a1) as a1' eqn:Heqa1'.
+    remember (fold_constants_aexp a2) as a2' eqn:Heqa2'.
+    replace (aeval st a1) with (aeval st a1') by
+       (subst a1'; rewrite <- fold_constants_aexp_sound; reflexivity).
+    replace (aeval st a2) with (aeval st a2') by
+       (subst a2'; rewrite <- fold_constants_aexp_sound; reflexivity).
+      destruct a1'; destruct a2'; try reflexivity.
+      simpl. destruct (n <=? n0); reflexivity.
   - (* BGt *)
-    (* FILL IN HERE *) admit.
+    simpl.
+    remember (fold_constants_aexp a1) as a1' eqn:Heqa1'.
+    remember (fold_constants_aexp a2) as a2' eqn:Heqa2'.
+    replace (aeval st a1) with (aeval st a1') by
+       (subst a1'; rewrite <- fold_constants_aexp_sound; reflexivity).
+    replace (aeval st a2) with (aeval st a2') by
+       (subst a2'; rewrite <- fold_constants_aexp_sound; reflexivity).
+      destruct a1'; destruct a2'; try reflexivity.
+      simpl. destruct (n <=? n0); reflexivity.
   - (* BNot *)
     simpl. remember (fold_constants_bexp b) as b' eqn:Heqb'.
     rewrite IHb.
@@ -1128,8 +1200,7 @@ Proof.
     remember (fold_constants_bexp b2) as b2' eqn:Heqb2'.
     rewrite IHb1. rewrite IHb2.
     destruct b1'; destruct b2'; reflexivity.
-(* FILL IN HERE *) Admitted.
-(** [] *)
+Qed.
 
 (** **** Exercise: 3 stars, standard (fold_constants_com_sound)
 
@@ -1159,8 +1230,14 @@ Proof.
       apply trans_cequiv with c2; try assumption.
       apply if_false; assumption.
   - (* while *)
-    (* FILL IN HERE *) Admitted.
-(** [] *)
+    assert (bequiv b (fold_constants_bexp b)). {
+      apply fold_constants_bexp_sound. }
+    destruct (fold_constants_bexp b) eqn:Heqb;
+      try (apply CWhile_congruence; assumption).
+    + apply while_true; assumption.
+    + apply while_false; assumption.
+Qed.
+  
 
 (* ================================================================= *)
 (** ** Soundness of (0 + n) Elimination, Redux *)
@@ -1404,8 +1481,7 @@ Proof.
 Theorem inequiv_exercise:
   ~ cequiv <{ while true do skip end }> <{ skip }>.
 Proof.
-  (* FILL IN HERE *) Admitted.
-(** [] *)
+  Search(cequiv _ <{ skip }>). Check while_false. apply while_false. destruct H.
 
 (* ################################################################# *)
 (** * Extended Exercise: Nondeterministic Imp *)
